ocaml/src/LoggerToSexp.mli
@@ -20,3 +20,4 @@ open SExp
    
 val logger_nra_to_sexp : Obj.t -> sexp
 val logger_nrc_to_sexp : Obj.t -> sexp
+val logger_dnrc_to_sexp : Obj.t -> sexp
