ocaml/src/Util.mli
@@ -23,6 +23,7 @@ exception Qcert_Error of string
 (* this can't go in Logger, since that creates a circular dependency *)
 type nra_logger_token_type = string
 type nrc_logger_token_type = string
+type dnrc_logger_token_type = string
 
 (**************)
 (* Data types *)
