coq/Compiler/CompilerModel/TrivialModel.v
@@ -22,6 +22,8 @@ Require Import ForeignCloudant ForeignToCloudant.
 Require Import CompilerRuntime CompilerModel.
 Require NNRCMR CloudantMR.
 Require Import OptimizerLogger String RAlgEnv NRAEnv NNRC.
+Require Import DNNRC Dataset.
+Require Import TDNRCInfer.
 
 Program Instance trivial_foreign_data : foreign_data
   := mk_foreign_data Empty_set _ _ _ _ _ _.
@@ -344,6 +346,8 @@ Existing Instance silent_optimizer_logger.
       := silent_optimizer_logger string nraenv.
     Definition compiler_nnrc_optimizer_logger : optimizer_logger string nnrc
       := silent_optimizer_logger string nnrc.
+    Definition compiler_dnnrc_optimizer_logger {br:brand_relation}: optimizer_logger string (dnnrc (type_annotation unit) dataset)
+      := silent_optimizer_logger string (dnnrc (type_annotation unit) dataset).
     Definition compiler_foreign_data_typing : foreign_data_typing
       := trivial_foreign_data_typing.
     
@@ -383,7 +387,9 @@ Existing Instance silent_optimizer_logger.
       := silent_optimizer_logger string nraenv.
     Definition compiler_model_nnrc_optimizer_logger : optimizer_logger string nnrc
       := silent_optimizer_logger string nnrc.
-    Definition compiler_model_foreign_data_typing : foreign_data_typing
+    Definition compiler_model_dnnrc_optimizer_logger {br:brand_relation}: optimizer_logger string (dnnrc (type_annotation unit) dataset)   
+      := silent_optimizer_logger string (dnnrc (type_annotation unit) dataset).
+ Definition compiler_model_foreign_data_typing : foreign_data_typing
       := trivial_foreign_data_typing.
   End TrivialModel.
 (* 
